cogent/llvm/checker/coq/Compiler.v
@@ -1,48 +1,108 @@
 From Coq Require Import List ZArith String.
 
-From ExtLib Require Import Data.Monads.StateMonad Structures.Monads Structures.Functor.
-From Vellvm Require Import LLVMAst.
+From ExtLib Require Import Structures.Monads Structures.Functor.
+From RecordUpdate Require Import RecordSet.
+From Vellvm Require Import LLVMAst Util.
 
-From Checker Require Import Cogent Types.
+From Checker Require Import Cogent Types State.
 
 Import ListNotations.
+Import RecordSetNotations.
+Import MonadNotation.
+Import FunctorNotation.
+Local Open Scope monad_scope.
 
 Section Compiler.
 
-  Import MonadNotation.
-  Import FunctorNotation.
-  Local Open Scope monad_scope.
-
   Definition CodegenValue : Type := texp typ.
-  (* Can't use record for state?: https://github.com/coq-community/coq-ext-lib/issues/48 *)
-  Definition CodegenState : Type := (code typ * Z * list (texp typ)).
-  Definition fresh : CodegenState -> Z := fun x => snd (fst x).
-  Definition blocks : CodegenState -> code typ := fun x => fst (fst x).
-  Definition vars : CodegenState -> list (texp typ) := snd.
+  Record CodegenState : Type := mk_state {
+    entry : block typ
+  ; blocks: list (block typ)
+  ; fresh_anon : Z
+  ; fresh_void : Z
+  ; fresh_block : Z
+  ; vars : list (texp typ)
+  }.
+  Instance etaCodegenState : Settable _ := settable! mk_state <
+    entry
+  ; blocks
+  ; fresh_anon
+  ; fresh_void
+  ; fresh_block
+  ; vars
+  >.
+
+  Instance etaBlock : Settable _ := settable! (@mk_block typ) <blk_id;blk_phis; blk_code; blk_term; blk_comments>.
+
+  Definition empty_block (n:block_id) : block typ :=
+    mk_block n [] [] (IVoid 0, TERM_Ret_void) None.
 
   Variable m : Type -> Type.
   Context {Monad_m: Monad m}.
   Context {State_m: MonadState CodegenState m}.
 
+  Definition current_block : m block_id :=
+    s <- get ;;
+    ret (blk_id (hd (entry s) (blocks s))).
+
+  Definition update_block (f:block typ -> block typ) (s:CodegenState) : CodegenState :=
+    match blocks s with
+    | [] => s <|entry := f (entry s)|>
+    | x :: xs => s <|blocks := f x :: xs|>
+    end.
+  
+  Definition new_block (n:block_id) : m unit :=
+    s <- get ;;
+    put (s <|blocks := empty_block n :: blocks s|>).
+  
+  Definition branch_blocks : m (block_id * block_id * block_id) :=
+    s <- get ;;
+    let n := fresh_block s in
+      put (s <|fresh_block := n + 1|>) ;;
+      ret (
+        Name ("if_" ++ string_of_Z n)
+      , Name ("then_" ++ string_of_Z n)
+      , Name ("done_" ++ string_of_Z n)
+      ).
 
   Definition instr (t:typ) (i:instr typ) : m CodegenValue :=
     s <- get ;;
-    let n := fresh s in
-      put (blocks s ++ [(IId (Anon n), i)], n + 1, vars s) ;;
+    let n := fresh_anon s in
+      put (
+        update_block (
+          fun x => x <|blk_code := blk_code x ++ [(IId (Anon n), i)]|>
+        ) s <|fresh_anon := n + 1|>
+      ) ;;
+      ret (t, EXP_Ident (ID_Local (Anon n))).
+
+  Definition term (t:terminator typ) : m unit :=
+    s <- get ;;
+    let n := fresh_void s in
+      put (update_block (fun x => x <|blk_term := (IVoid n, t)|>) s <|fresh_void := n + 1|>) ;;
+      ret tt.
+  
+  Definition phi (t:typ) (args:list (block_id * exp typ)) : m CodegenValue :=
+    s <- get ;;
+    let n := fresh_anon s in
+      put (
+        update_block (
+          fun x => x <|blk_phis := blk_phis x ++ [(Anon n, Phi t args)]|>
+        ) s <|fresh_anon := n + 1|>
+      ) ;;
       ret (t, EXP_Ident (ID_Local (Anon n))).
   
   Definition set_vars (vs:list (texp typ)) : m unit :=
     s <- get ;;
-    put (blocks s, fresh s, vs).
+    put (s <|vars := vs|>).
 
-  Definition compile_prim_op (o:prim_op) : (ibinop * typ * typ) :=
+  Definition compile_prim_op (o:prim_op) : (exp typ -> exp typ -> exp typ) * typ :=
     match o with
-    | Plus t => (Add false false, convert_num_type t, convert_num_type t)
-    | Minus t => (Sub false false, convert_num_type t, convert_num_type t)
-    | Times t => (Mul false false, convert_num_type t, convert_num_type t)
-    | Divide t => (UDiv false, convert_num_type t, convert_num_type t)
-    | Mod t => (URem, convert_num_type t, convert_num_type t)
-    | _ => (Xor, TYPE_Void, TYPE_Void)
+    | Plus t => (OP_IBinop (Add false false) (convert_num_type t), convert_num_type t)
+    | Minus t => (OP_IBinop (Sub false false) (convert_num_type t), convert_num_type t)
+    | Times t => (OP_IBinop (Mul false false) (convert_num_type t), convert_num_type t)
+    | Divide t => (OP_IBinop (UDiv false) (convert_num_type t), convert_num_type t)
+    | Mod t => (OP_IBinop URem (convert_num_type t), convert_num_type t)
+    | _ => (OP_IBinop Xor TYPE_Void, TYPE_Void)
     (* | Not 
     | And 
     | Or
@@ -65,17 +125,35 @@ Section Compiler.
   Fixpoint compile_expr (e:expr) : m CodegenValue :=
     match e with
     | Prim op [oa; ob] =>
-        let '(op', t, rt) := compile_prim_op op in
+        let (op', rt) := compile_prim_op op in
         va <- snd <$> compile_expr oa ;;
         vb <- snd <$> compile_expr ob ;;
-        instr rt (INSTR_Op (OP_IBinop op' t va vb)) 
+        instr rt (INSTR_Op (op' va vb)) 
     | Lit l => ret match l with
-      | LBool b => (TYPE_I 8, EXP_Integer (if b then 1 else 0))
+      | LBool b => (TYPE_I 1, EXP_Integer (if b then 1 else 0))
       | LU8 w => (TYPE_I 8, EXP_Integer w)
       | LU16 w => (TYPE_I 16, EXP_Integer w)
       | LU32 w => (TYPE_I 32, EXP_Integer w)
       | LU64 w => (TYPE_I 64, EXP_Integer w)
       end
+    | Unit => ret (TYPE_I 2, EXP_Integer 0)
+    | If c b1 b2 =>
+        c' <- compile_expr c ;;
+        '(br_true, br_false, br_exit) <- branch_blocks ;;
+        term (TERM_Br c' br_true br_false) ;;
+
+        new_block br_true ;;
+        b1' <- compile_expr b1 ;;
+        br_true' <- current_block ;;
+        term (TERM_Br_1 br_exit) ;;
+
+        new_block br_false;;
+        b2' <- compile_expr b2 ;;
+        br_false' <- current_block ;;
+        term (TERM_Br_1 br_exit) ;;
+
+        new_block br_exit ;;
+        phi (fst b1') [(br_true', snd b1'); (br_false', snd b2')]
     | Var i =>
         s <- get ;;
         ret (nth i (vars s) undef)
@@ -100,17 +178,24 @@ Section Compiler.
     | _ => TYPE_Void
     end.
 
-  Definition startState: CodegenState := ([], 0, []).
+  Definition start_state (t:typ) : CodegenState := {|
+    entry := empty_block (Name "entry_0")
+  ; blocks := []
+  ; fresh_anon := 0
+  ; fresh_void := 0
+  ; fresh_block := 0
+  ; vars := [(t, EXP_Ident (ID_Local (Name "a_0")))]
+  |}.
 
 End Compiler.
 
-Definition build_expr (p:expr) : CodegenValue * CodegenState :=
-  runState (compile_expr (state CodegenState) p) startState.
+Definition build_expr (p:expr) (t:type) : CodegenState :=
+  execState (v <- compile_expr _ p ;; term _ (TERM_Ret v)) (start_state (compile_type t)).
 
 Definition compile_def (d:def) : toplevel_entity typ (block typ * list (block typ)) :=
   match d with
   | FunDef n t rt b => 
-      let (value, state) := build_expr b in  
+      let state := build_expr b t in  
         TLE_Definition {|
           df_prototype := {|
             dc_name := Name n
@@ -125,12 +210,6 @@ Definition compile_def (d:def) : toplevel_entity typ (block typ * list (block ty
           ; dc_align := None
           ; dc_gc := None|}
         ; df_args := [(Name "a_0")]
-        ; df_instrs := ({|
-            blk_id := Name "entry_0"
-          ; blk_phis := []
-          ; blk_code := blocks state
-          ; blk_term := (IVoid 0, TERM_Ret value)
-          ; blk_comments := None
-          |}, [])
+        ; df_instrs := (entry state, rev (blocks state))
         |}
   end.
