cogent/llvm/checker/coq/State.v
@@ -1,0 +1,40 @@
+(* See: https://github.com/coq-community/coq-ext-lib/issues/48 *)
+
+Require Import ExtLib.Structures.Monads.
+Require Import ExtLib.Structures.Monoid.
+
+Set Implicit Arguments.
+Set Strict Implicit.
+Set Primitive Projections.
+Set Universe Polymorphism.
+
+Section StateType.
+  Variable S : Type.
+
+  Record state (t : Type) : Type := mkState
+  { runState : S -> t * S }.
+
+  Definition evalState {t} (c : state t) (s : S) : t :=
+    fst (runState c s).
+
+  Definition execState {t} (c : state t) (s : S) : S :=
+    snd (runState c s).
+
+
+  Global Instance Monad_state : Monad state :=
+  { ret  := fun _ v => mkState (fun s => (v, s))
+  ; bind := fun _ _ c1 c2 =>
+    mkState (fun s =>
+      let (v,s) := runState c1 s in
+      runState (c2 v) s)
+  }.
+
+  Global Instance MonadState_state : MonadState S state :=
+  { get := mkState (fun x => (x,x))
+  ; put := fun v => mkState (fun _ => (tt, v))
+  }.
+
+End StateType.
+
+Arguments evalState {S} {t} (c) (s).
+Arguments execState {S} {t} (c) (s).
